test/TheoryTest.v
@@ -1,0 +1,668 @@
+(*Here, we manually instantiate a few theories to test
+  that (especially) the cloning/qualifying works*)
+Require Import Task.
+Require Import Theory.
+Require Import Typechecker.
+From mathcomp Require Import all_ssreflect.
+Set Bullet Behavior "Strict Subproofs".
+
+(*Why3 has constants, which so far as I can tell are just
+  function symbols that take no arguments. We give some
+  utilities*)
+Definition mk_constant (name: string) (ty: vty):=
+  Build_funsym (Build_fpsym name nil nil erefl erefl) ty.
+
+
+(*Here, we first use some examples from why3/stdlib/algebra*)
+
+Module Alg.
+
+Definition t : typesym := mk_ts "t" nil.
+Definition t_ty : vty := vty_cons t nil.
+
+Definition op: funsym := Build_funsym 
+  (Build_fpsym "op" nil [t_ty; t_ty] erefl erefl)
+  t_ty erefl.
+
+Definition x : vsymbol := ("x"%string, t_ty).
+Definition y : vsymbol := ("y"%string, t_ty).
+Definition z : vsymbol := ("z"%string, t_ty).
+
+Module Assoc.
+
+Definition assoc : theory :=
+  rev [
+    (*type t*)
+    tdef (abs_type t);
+    (*function op t t : t*)
+    tdef (abs_fun op);
+    (*axiom Assoc : forall x y z : t. op (op x y) z = op x (op y z)*)
+    tprop Paxiom "Assoc" (fforalls [x; y; z]
+      (Feq t_ty (Tfun op nil [Tfun op nil [Tvar x; Tvar y]; Tvar z])
+        (Tfun op nil [Tvar x; Tfun op nil [Tvar y; Tvar z]])))
+  ].
+
+Lemma assoc_typed : typed_theory assoc.
+Proof.
+  check_theory.
+Qed.
+
+Lemma assoc_valid: valid_theory assoc.
+Proof.
+  simpl. split; auto. prove_task_wf.
+Qed.
+
+End Assoc.
+
+(*Commutativity*)
+Module Comm.
+
+Definition comm: theory :=
+  rev [
+    (*type t*)
+    tdef (abs_type t);
+    (*function op t t : t*)
+    tdef (abs_fun op);
+    (*axiom Comm : forall x y : t. op x y = op y x*)
+    tprop Paxiom "Comm" (fforalls [x; y]
+      (Feq t_ty (Tfun op nil [Tvar x; Tvar y]) 
+        (Tfun op nil [Tvar y; Tvar x])))
+  ].
+
+Definition comm_typed : typed_theory comm.
+Proof.
+  check_theory. 
+Qed.
+
+Lemma comm_valid: valid_theory comm.
+Proof.
+  simpl. split; auto. prove_task_wf.
+Qed.
+
+End Comm.
+
+(*Monoid*)
+Module Monoid.
+
+Definition unit : funsym := mk_constant "unit" t_ty erefl.
+
+Definition monoid : theory :=
+  rev [
+    (*clone export Assoc*)
+    tclone Assoc.assoc None nil nil nil;
+    (*constant unit : t*)
+    tdef (abs_fun unit);
+    (*axiom Unit_def_l : forall x:t. op unit x = x*)
+    tprop Paxiom "Unit_def_l" (Fquant Tforall x (Feq t_ty 
+      (Tfun op nil [Tfun unit nil nil; Tvar x]) (Tvar x)));
+    (*axiom Unit_def_r : forall x:t. op x unit = x*)
+    tprop Paxiom "Unit_def_r" (Fquant Tforall x (Feq t_ty
+      (Tfun op nil [Tvar x; Tfun unit nil nil]) (Tvar x)))
+  ].
+
+Lemma monoid_ctx : theory_ctx_int monoid =
+  rev [abs_type t; abs_fun op; abs_fun unit].
+Proof.
+  reflexivity.
+Qed.
+
+Lemma monoid_valid: valid_theory monoid.
+Proof.
+  simpl; split_all; auto; prove_task_wf.
+Qed.
+
+Lemma monoid_typed: typed_theory monoid.
+Proof. check_theory. Qed.
+
+End Monoid.
+
+(*Commutative Monoid*)
+
+Module CommutativeMonoid.
+
+Definition comm_monoid : theory :=
+  rev [
+    (*clone export Monoid*)
+    tclone Monoid.monoid None nil nil nil;
+    (*clone export Comm with type t = t, function op = op*)
+    tclone Comm.comm None [(t, t)] [(op, op)] nil
+  ].
+
+(*Still same context*)
+Lemma comm_monoid_ctx : theory_ctx_int comm_monoid =
+rev [abs_type t; abs_fun op; abs_fun Monoid.unit].
+Proof.
+  reflexivity.
+Qed.
+
+Lemma comm_monoid_typed: typed_theory comm_monoid.
+Proof. check_theory. Qed.
+
+Lemma comm_monoid_valid: valid_theory comm_monoid.
+Proof.
+  simpl; split_all; auto; prove_task_wf.
+Qed.
+
+End CommutativeMonoid.
+
+(*Group*)
+
+Module Group.
+
+Definition inv : funsym := Build_funsym 
+  (Build_fpsym "inv" nil [t_ty] erefl erefl) t_ty erefl.
+
+Definition group : theory :=
+  rev [
+    (*clone export Monoid*)
+    tclone Monoid.monoid None nil nil nil;
+    (*function inv t : t*)
+    tdef (abs_fun inv);
+    (*axiom Inv_def_l : forall x:t. op (inv x) x = unit*)
+    tprop Paxiom "Inv_def_l" (Fquant Tforall x (Feq t_ty 
+      (Tfun op nil [Tfun inv nil [Tvar x]; Tvar x]) (Tfun Monoid.unit nil nil)));
+    (*axiom Inv_def_r : forall x:t. op x (inv x) = unit*)
+    tprop Paxiom "Inv_def_r" (Fquant Tforall x (Feq t_ty
+      (Tfun op nil [Tvar x; Tfun inv nil [Tvar x]]) (Tfun Monoid.unit nil nil)))
+  ].
+
+(*Now, we have inverse*)
+Lemma group_ctx : theory_ctx_int group =
+rev [abs_type t; abs_fun op; abs_fun Monoid.unit;
+  abs_fun inv].
+Proof.
+  reflexivity.
+Qed.
+
+Lemma group_typed: typed_theory group.
+Proof. check_theory. Qed.
+
+Lemma group_valid: valid_theory group.
+Proof.
+  simpl; split_all; auto; prove_task_wf.
+Qed.
+
+
+End Group.
+
+(*Commutative Groups*)
+Module CommGroup.
+
+Definition comm_group : theory :=
+  rev [
+    (*clone export Group*)
+    tclone Group.group None nil nil nil;
+    (*clone export Comm with type t = t, function op = op*)
+    tclone Comm.comm None [(t, t)] [(op, op)] nil
+  ].
+
+Lemma comm_group_ctx : theory_ctx_int comm_group =
+rev [abs_type t; abs_fun op; abs_fun Monoid.unit;
+  abs_fun Group.inv].
+Proof.
+  reflexivity.
+Qed.
+
+Lemma comm_group_typed: typed_theory comm_group.
+Proof. check_theory. Qed.
+
+Lemma comm_group_valid: valid_theory comm_group.
+Proof.
+  simpl; split_all; auto; prove_task_wf.
+Qed.
+
+End CommGroup.
+
+(*Rings*)
+
+Module Ring.
+
+(*Here, things get a bit interesting, since we have multiple
+  clones and more than 1 set of functions interacting.
+  We do not support the infix notation of why3*)
+
+Definition zero : funsym := mk_constant "zero" t_ty erefl.
+Definition plus : funsym := Build_funsym 
+  (Build_fpsym "plus" nil [t_ty; t_ty] erefl erefl)
+  t_ty erefl.
+Definition mult : funsym := Build_funsym 
+  (Build_fpsym "mult" nil [t_ty; t_ty] erefl erefl)
+  t_ty erefl.
+Definition neg : funsym := Build_funsym 
+(Build_fpsym "neg" nil [t_ty] erefl erefl)
+t_ty erefl.
+
+(*Unlike regular why3, we require qualified names in "clone"*)
+Definition MA_t : typesym := mk_ts "MulAssoc.t" nil.
+Definition MA_t_ty : vty := vty_cons MA_t nil.
+(*We have utilities to do this, but we are testing them, so we
+  do it by hand*)
+Definition MA_op: funsym := Build_funsym (Build_fpsym "MulAssoc.op" nil [MA_t_ty; MA_t_ty] erefl erefl)
+  MA_t_ty erefl.
+
+Definition ring : theory :=
+  rev [
+    (*type t*)
+    tdef (abs_type t);
+    (*constant zero : t*)
+    tdef (abs_fun zero);
+    (*function (+) t t : t*)
+    tdef (abs_fun plus);
+    (*function (-_) t : t*)
+    tdef (abs_fun neg);
+    (*function ( * ) t t: t*)
+    tdef (abs_fun mult);
+    (*clone export CommutativeGroup with type t = t,
+                                constant unit = zero,
+                                function op = (+),
+                                function inv = (-_)*)
+    tclone CommGroup.comm_group None [(t, t)] [(Monoid.unit, zero); 
+      (op, plus); (Group.inv, neg)] nil;
+    (*clone Assoc as MulAssoc with type t = t, function op = ( * )*)
+    tclone Assoc.assoc (Some "MulAssoc"%string) [(MA_t, t)] [(MA_op, mult)] nil;
+    (*axiom Mul_distr_l : forall x y z : t. x * (y + z) = x * y + x * z*)
+    tprop Paxiom "Mul_distr_l" (fforalls [x; y; z] (Feq t_ty
+      (Tfun mult nil [Tvar x; Tfun plus nil [Tvar y; Tvar z]])
+      (Tfun plus nil [Tfun mult nil [Tvar x; Tvar y]; Tfun mult nil [Tvar x; Tvar z]])
+    ));
+    (*axiom Mul_distr_r : forall x y z : t. (y + z) * x = y * x + z * x*)
+    tprop Paxiom "Mul_distr_r" (fforalls [x;y;z] (Feq t_ty
+      (Tfun mult nil [Tfun plus nil [Tvar y; Tvar z]; Tvar x])
+      (Tfun plus nil [Tfun mult nil [Tvar y; Tvar x]; Tfun mult nil [Tvar z; Tvar x]])
+    ))
+  ].
+
+(*Note that all of our exports do not add to the context. This fails
+  if we don't add the qualified names in the "with" part*)
+Lemma ring_ctx : theory_ctx_int ring =
+rev [abs_type t; abs_fun zero; abs_fun plus; abs_fun neg; abs_fun mult].
+Proof.
+  reflexivity.
+Qed.
+
+(*The context (with the qualified names and everything)
+  is still well-typed (meaning so are all the lemmas)*)
+Lemma ring_typed: typed_theory ring.
+Proof. check_theory. Qed.
+
+(*god Coq is annoying sometimes*)
+
+Lemma all_cons {T: Type} (p: pred T) (h: T) (s: seq T):
+  all p (h :: s) = p h && all p s.
+Proof.
+  reflexivity.
+Qed.
+
+(*Problem - we cannot typecheck the context: why
+  we have (from assoc)
+  - forall x y z, (x op y) op z = x op (y op z)
+  (from other assoc)
+  - 
+
+*)
+(*
+Lemma ring_valid: valid_theory ring.
+Proof.
+  simpl; split_all; auto; try prove_task_wf.
+  - (*OK, what is problem here?*)
+    apply /check_task_wf_correct.
+    unfold check_task_wf.
+    apply /andP; split; auto.
+    apply /andP; split; auto.
+    apply /andP; split; auto.
+    apply /andP; split; auto.
+    apply /andP; split; auto.
+    + simpl task_delta.
+      rewrite all_cons. apply /andP. split; auto.
+      unfold Assoc.assoc, rev, catrev.
+      rewrite !get_exported_names_equation_3.
+      rewrite !get_exported_names_equation_2.
+      rewrite get_exported_names_equation_1.
+      rewrite qualify_theory_equation_3.
+      rewrite !qualify_theory_equation_2.
+      rewrite qualify_theory_equation_1.
+      simpl.
+      rewrite theory_axioms_ext_equation_4.
+      rewrite !theory_axioms_ext_equation_2.
+      rewrite theory_axioms_ext_equation_1.
+      unfold sub_props_map. simpl List.map.
+      simpl map.
+      rewrite all_cons.
+      apply /andP; split; auto.
+      (*Aha, so this one is the problem*)
+      apply /typecheck_formula_correct.
+      apply F_Quant; auto.
+      {
+        apply /typecheck_type_correct. reflexivity.
+      }
+      simpl. apply F_Quant; auto.
+      {
+        apply /typecheck_type_correct. reflexivity.
+      }
+      simpl. apply F_Quant; auto.
+      {
+        apply /typecheck_type_correct. reflexivity.
+      }
+      apply F_Eq.
+      {
+        (*A problem here - why is everything op?*)
+        apply T_Fun; simpl; auto.
+        - apply /inP. reflexivity.
+        - apply /typecheck_type_correct. reflexivity.
+        -
+        
+        
+        repeat constructor; auto. apply /forallb_ForallP. reflexivity. unfold CommGroup.comm_group, Group.group, Comm.comm, Monoid.monoid, Assoc.assoc,
+        rev, catrev. 
+          simpl. rewrite !theory_ctx_ext_equation_3.
+          rewrite !theory_ctx_ext_equation_2.
+          rewrite theory_ctx_ext_equation_1.
+          simpl.
+          rewrite !theory_ctx_ext_equation_6.
+          simpl.
+          rewrite theory_ctx_ext_equation_1.
+          simpl.
+          rewrite !theory_ctx_ext_equation_3.
+          rewrite !theory_ctx_ext_equation_2.
+          rewrite !theory_ctx_ext_equation_6. simpl.
+          rewrite !theory_ctx_ext_equation_3.
+          rewrite !theory_ctx_ext_equation_2.
+          rewrite !theory_ctx_ext_equation_6. simpl.
+          rewrite !theory_ctx_ext_equation_3.
+          rewrite !theory_ctx_ext_equation_2.
+          rewrite !theory_ctx_ext_equation_1.
+          rewrite !app_nil_r.
+
+          simpl sig_f. unfold sig_f. simpl List.map.
+          unfold sub_funs.
+          unfold sub_from_map.
+          simpl get_assoc_list. simpl. auto.
+          (*WTF, this is true. What is going on?*)
+          simpl sub_funs.
+          unfold sub_funs. simpl.
+          unfold sub_ctx_map. simpl.
+          unfold Group.grou
+          simpl.
+          unfold sub_ctx_map.
+          
+          u
+
+        apply /typecheck_term_correct. reflexivity.
+      }
+      simpl.
+      simpl.
+      unfold qual_fmla.
+      unfold sub_in_f.
+      simpl.
+      simpl.
+      reflexivity.
+
+
+      rewrite all_cons.
+      rewrite all_cons.
+      simpl.
+      
+      simpl.
+
+      unfold sub_props_map.
+      simpl.
+    
+    simpl.
+    
+    
+    reflexivity.
+    
+    
+    simpl.
+    
+    simpl.
+
+
+Qed.
+*)
+End Ring.
+
+(*Now, we prove a few simple theories (manually)
+  about rings. This is not part of the stdlib (names from
+  mathcomp)*)
+Module RingTheory.
+
+Definition ring_theory : theory :=
+  rev [
+    (*use ring*)
+    tuse Ring.ring false;
+    (*lemma subr0_eq : forall x y : t. x + (- y) = 0 -> x = y*)
+    tprop Plemma "subr0_eq" (fforalls [x; y] (Fbinop Timplies
+      (Feq t_ty (Tfun Ring.plus nil [Tvar x; Tfun Ring.neg nil [Tvar y]]) (Tfun Ring.zero nil nil))
+      (Feq t_ty (Tvar x) (Tvar y))  
+    ));
+    (*lemma add_cancel_l: forall x y z: t. x + y = x + z -> y = z*)
+    tprop Plemma "add_cancel_l" (fforalls [x;y;z] (Fbinop Timplies
+      (Feq t_ty (Tfun Ring.plus nil [Tvar x; Tvar y])
+        (Tfun Ring.plus nil [Tvar x; Tvar z]))
+      (Feq t_ty (Tvar y) (Tvar z))
+    ));
+    (*lemma mulr0: forall x: t. x * 0 = 0*)
+    tprop Plemma "mulr0" (Fquant Tforall x (Feq t_ty
+      (Tfun Ring.mult nil [Tvar x; Tfun Ring.zero nil nil])
+      (Tfun Ring.zero nil nil)))
+  ].
+
+(*Internal context still has everything from ring*)
+Lemma ring_theory_ctx : theory_ctx_int ring_theory =
+rev [abs_type t; abs_fun Ring.zero; abs_fun Ring.plus; abs_fun Ring.neg; abs_fun Ring.mult].
+Proof.
+  reflexivity.
+Qed.
+
+(*External context is empty*)
+Lemma ring_theory_ctx_ext: theory_ctx_ext ring_theory = nil.
+Proof.
+  reflexivity.
+Qed.
+
+(*Everything is well-typed*)
+Lemma ring_theory_typed: typed_theory ring_theory.
+Proof. check_theory. Qed.
+
+
+
+(*Now, we prove these lemmas (manually, from the semantics)
+  *)
+  (*
+Lemma ring_theory_valid: valid_theory ring_theory.
+Proof.
+  simpl. split_all; auto.
+  - (*First lemma*)
+    unfold task_valid. simpl. split.
+    +  apply /check_task_wf_correct.
+
+      unfold check_task_wf.  
+      assert (check_context (theory_ctx_ext Ring.ring ++ [::])%list).
+        reflexivity.
+      rewrite H.
+      do 5 (try (apply /andP; split)); auto.
+      unfold task_delta.
+      rewrite all_cons.
+      apply /andP. split; auto.
+      rewrite all_cons. apply /andP. split; try reflexivity.
+      (*This is the hard one - one that doesnt work*)
+      rewrite theory_axioms_ext_equation_1.
+      rewrite !app_nil_r.
+      (*This should follow from above?*)
+      unfold Ring.ring.
+      unfold rev, catrev.
+      rewrite theory_axioms_ext_equation_4.
+      rewrite theory_axioms_ext_equation_4.
+      rewrite theory_axioms_ext_equation_8.
+      rewrite theory_axioms_ext_equation_8.
+      rewrite theory_axioms_ext_equation_2.
+      rewrite theory_axioms_ext_equation_2.
+      rewrite theory_axioms_ext_equation_2.
+      rewrite theory_axioms_ext_equation_2.
+      rewrite theory_axioms_ext_equation_2.
+      rewrite theory_axioms_ext_equation_1.
+      reflexivity.
+      unfold Assoc.assoc.
+      rewrite app_nil_r.
+      rewrite all_cons. unfold is_true. rewrite andb_true_iff. split; try reflexivity.
+
+      * reflexivity.
+      *
+      
+      apply /andP.
+      idtac.
+      reflexivity.
+      
+
+
+      rewrite !all_cons.
+      unfold is_true.
+      Search all cons.
+      simpl all.
+      cbn iota.
+      rewrite andb_true_iff.
+      apply /andP; split.
+      * reflexivity.
+      * unfold Ring.ring. unfold rev. unfold catrev.
+        rewrite theory_axioms_ext_equation_4.
+        cbn beta. unfold is_true. rewrite andb_true_iff.
+        split; try reflexivity.
+        unfold is_true.
+        cbn.
+
+        rewrite andb_true_iff. split; try reflexivity.
+
+      
+      
+      simpl catrev. simpl rev.
+      
+      
+      simpl. unfold theory_ctx_ext. apply /andP. split; try reflexivity.
+
+
+        simpl.
+        repeat (apply /andP; split; try reflexivity). idtac.
+        unfold sub_tys. unfold sub_from_map. simpl.
+
+        unfold get_exported_names.
+
+
+        reflexivity.
+        
+        reflexivity.
+      
+      unfold Ring.ring. simpl. reflexivity. apply /andP. split; try reflexivity.
+        simpl. rewrite -/all. simpl. rewrite -andbA. simpl. apply /andP. 
+
+
+      simpl.
+      simpl all.
+      simpl.
+      reflexivity.
+      compute.
+      simpl.
+
+
+      apply /andP. split.
+      rewrite <- !andbA.
+      do 3 (try (apply /andP; split)).
+      * auto.
+      * reflexivity.
+      * reflexivity.
+      repeat (apply /andP; split).
+      simpl.
+    
+    simpl.
+    reflexivity.
+    
+    prove_task_wf. *)
+
+(*Plan: prove cancellation, zero identity in ring*)
+
+(*THEN, do unit ring*)
+
+(*then prove 1 results about mult and -1*)
+
+(*Now, as a quick test, we prove some theorems about rings*)
+
+
+(*TODO: groups, comm groups, rings
+  Then, prove some ring theorems*)
+
+(*old, maybe get rid of after finishing ring theory*)
+(*Here, a simple test for cloning with a name and
+  substitution - fixed some bugs in Theory with this*)
+  (*Much simpler test*)
+  Module Test.
+
+  Definition theory1 : theory :=
+    rev [
+      tdef (abs_type t);
+      tdef (abs_fun op)
+    ].
+  (*Unlike why3, we require qualified names even in clone declaration*)
+  Definition tt : typesym := mk_ts "T.t" nil.
+  Definition tt_ty : vty := vty_cons tt nil.
+  Definition top : funsym := Build_funsym (Build_fpsym "T.op" nil [tt_ty; tt_ty] erefl erefl)
+    tt_ty erefl.
+  
+  Definition theory2 : theory :=
+    rev [
+      tdef (abs_type t);
+      tdef (abs_fun op);
+      tclone theory1 (Some "T"%string) [(tt, t)] [(top, op)] nil;
+      tprop Paxiom "foo" (fforalls [x; y] (Feq t_ty
+        (Tfun op nil [Tvar x; Tvar y])
+        (Tfun op nil [Tvar y; Tvar x])
+      ))
+    ].
+  
+  Lemma theory2_ctx: theory_ctx_int theory2 =
+    rev [abs_type t; abs_fun op].
+  Proof. reflexivity. Qed.
+  
+  Lemma theory2_ctx_ext: theory_ctx_ext theory2 =
+  rev [abs_type t; abs_fun op].
+  Proof.
+    reflexivity.
+  Qed.
+  
+  (*Typed*)
+  Lemma theory2_typed: typed_theory theory2.
+  Proof.
+    check_theory.
+  Qed.
+  
+  (*Well-formed*)
+  Lemma theory2_valid: valid_theory theory2.
+  Proof.
+    simpl. split; auto. prove_task_wf.
+  Qed.
+
+
+(*Test where we clone twice*)
+
+
+(*TODO: start here*)
+(*Want to see why we have issues in ring
+  I think - has to do with same module being cloned twice
+  Try: module with axiom, clone twice with different ops and names
+  then try with 1 that is unqualified
+  see if we find an issue
+  *)
+
+  Definition theory3 : theory :=
+    rev [
+      tdef (abs_type t);
+      tdef (abs_fun Ring.plus);
+      tdef (abs_fun Ring.mult);
+      tclone theory2 (Some "T"%string) [(tt, t)] [(top, plus)] nil;
+      tclone theory2 (Some "A"%string) []
+      tprop Paxiom "foo" (fforalls [x; y] (Feq t_ty
+        (Tfun op nil [Tvar x; Tvar y])
+        (Tfun op nil [Tvar y; Tvar x])
+      ))
+    ].
+  
+  End Test.
